tests/testMemoryModelScript.sml
@@ -1,14 +1,17 @@
+open HolKernel Parse boolLib bossLib;
 
-(*load "uvmThreadSemanticsTheory";*)
-load "uvmMemoryModelTheory";
+load "../uvmMemoryModelTheory";
 open uvmMemoryModelTheory;
 open uvmIRTheory;
 
+val _ = new_theory "testMemoryModel";
 
 (*___  ___ ___ ___ _  _ ___ _____ ___ ___  _  _ ___ 
  |   \| __| __|_ _| \| |_ _|_   _|_ _/ _ \| \| / __|
  | |) | _|| _| | || .` || |  | |  | | (_) | .` \__ \
  |___/|___|_| |___|_|\_|___| |_| |___\___/|_|\_|___/ *)
+
+(* {{{ *)
 
 (* I define an alternate receive that's not a relation *)
 val receive' = Define`
@@ -43,16 +46,32 @@ val dataRace_def = Define`
 val unsequencedRace_def = Define`
     unsequencedRace g A B = (
        (sameThread A B)              ∧
-       (sameAddress A B)            ∧
+       (sameAddress A B)             ∧
        ( (isStore A) ∨ (isStore B) ) ∧
       ~(sequencedBefore g A B)       ∧
       ~(sequencedBefore g B A)
 )`;
 
 
+val n = Define`n m = (Int m 8)`;
+
+(* sameAddress *)
+val ad_sanity_0 = prove( ``∀nd. (sameAddress nd nd)``, EVAL_TAC THEN RW_TAC (srw_ss()) []);
 
 
 
+Define `g0= FOLDL (receive') empty
+         [
+            ( Write 10 0 (n 11) NOT_ATOMIC {} , 0) ;
+            ( Read  10 1        SEQ_CST    {} , 1) ;
+            ( Write 10 2 (n 12) SEQ_CST    {} , 1) ;
+            ( Write 10 3 (n 13) NOT_ATOMIC {} , 1)
+         ]`;
+Define `w0_0 = (EL 0 g0.nodes)`; Define `r0_1 = (EL 1 g0.nodes)`; Define `w0_2 = (EL 2 g0.nodes)`;
+Define `w0_3 = (EL 3 g0.nodes)`;
+
+
+(* }}} *)
 
 
 
@@ -61,13 +80,7 @@ val unsequencedRace_def = Define`
   / _ \ '_/ _` / -_) '_/ -_) _` | _ \/ -_)  _/ _ \ '_/ -_)
   \___/_| \__,_\___|_| \___\__,_|___/\___|_| \___/_| \___|  *)
 
-Define `g0= FOLDL (receive') empty
-         [
-            ( Write 1024 0 112 NOT_ATOMIC {} , 0) ;
-            ( Read  1024 1     SEQ_CST    {} , 1) ;
-            ( Write 1024 2 10  SEQ_CST    {} , 1)
-         ]`;
-Define `w0_0 = (EL 0 g0.nodes)`; Define `r0_1 = (EL 1 g0.nodes)`; Define `w0_2 = (EL 2 g0.nodes)`;
+(* {{{ *)
 
 (* Specific *)
 val ob_eg0 = prove(``orderedBefore g0 r0_1 w0_2``, EVAL_TAC);
@@ -85,24 +98,18 @@ val ob_gen5 = prove(
     ``∀ g nd1 nd2 nd3. ((orderedBefore g nd1 nd2) ∧ (orderedBefore g nd2 nd3)) ==> (orderedBefore g nd1 nd3)``,
         RW_TAC arith_ss [orderedBefore_def]);
 
+(* }}} *)
 
 (* _ __  ___  __| (_)/ _(_)___ __| _ ) ___ / _|___ _ _ ___ 
   | '  \/ _ \/ _` | |  _| / -_|_-< _ \/ -_)  _/ _ \ '_/ -_)
   |_|_|_\___/\__,_|_|_| |_\___/__/___/\___|_| \___/_| \___|  *)
 
-Define `g1= FOLDL (receive') empty
-         [
-            ( Write 1024 0 112 NOT_ATOMIC {} , 0) ;
-            ( Write 9999 1 112 NOT_ATOMIC {} , 0) ;
-            ( Write 1024 2 112 NOT_ATOMIC {} , 1) ;
-            ( Read  1024 4     SEQ_CST    {} , 0) 
-         ]`;
-Define `w1_0 = (EL 0 g1.nodes)`; Define `w1_1 = (EL 1 g1.nodes)`;
-Define `w1_2 = (EL 2 g1.nodes)`; Define `r1_3 = (EL 3 g1.nodes)`;
+(* {{{ *)
 
-val mb_eg0 = prove(``modifiesBefore g1 w1_0 w1_2``, EVAL_TAC);
-val mb_eg1 = prove(``~modifiesBefore g1 w1_0 w1_1``, EVAL_TAC);
-val mb_eg2 = prove(``~modifiesBefore g1 w1_0 r1_3``, EVAL_TAC);
+val mb_eg0 = prove(`` modifiesBefore g0 w0_2 w0_3``, EVAL_TAC);
+val mb_eg1 = prove(`` modifiesBefore g0 w0_0 w0_2``, EVAL_TAC);
+val mb_eg2 = prove(``~modifiesBefore g0 w0_0 r0_1``, EVAL_TAC);
+val mb_eg2 = prove(`` modifiesBefore g0 w0_0 w0_3``, EVAL_TAC);
 
 val mb_general3 = prove(
     ``∀ g nd. ~modifiesBefore g nd nd``,
@@ -111,29 +118,31 @@ val mb_general4 = prove(
     ``∀ g nd1 nd2. (modifiesBefore g nd1 nd2) ==> ~(modifiesBefore g nd2 nd1)``,
     RW_TAC arith_ss [modifiesBefore_def,orderedBefore_def,sameAddress_def]);
 
+(* }}} *)
 
 (* ___ ___ __ _ _  _ ___ _ _  __ ___ __| | _ ) ___ / _|___ _ _ ___ 
   (_-</ -_) _` | || / -_) ' \/ _/ -_) _` | _ \/ -_)  _/ _ \ '_/ -_)
   /__/\___\__, |\_,_\___|_||_\__\___\__,_|___/\___|_| \___/_| \___|
             |_|                                                    *)
+(* {{{ *)
 
 Define `g2= FOLDL (receive') empty
          [                                            (* int main() {   *)
-           ( Write 10 0 2 NOT_ATOMIC    {} , 1 ) ;    (*   int x = 2    *)
-           ( Write 20 1 0 NOT_ATOMIC    {} , 1 ) ;    (*   int y = 0    *)
-           ( Read  10 2   NOT_ATOMIC    {} , 1 ) ;    (*   y = (x == x) *)
-           ( Read  10 3   NOT_ATOMIC    {} , 1 ) ;
-           ( Write 20 4 1 NOT_ATOMIC {2;3} , 1 )
+           ( Write 10 0 (n 2) NOT_ATOMIC    {} , 1 ) ;    (*   int x = 2    *)
+           ( Write 20 1 (n 0) NOT_ATOMIC    {} , 1 ) ;    (*   int y = 0    *)
+           ( Read  10 2       NOT_ATOMIC    {} , 1 ) ;    (*   y = (x == x) *)
+           ( Read  10 3       NOT_ATOMIC    {} , 1 ) ;
+           ( Write 20 4 (n 1) NOT_ATOMIC {2;3} , 1 )
          ]`;                                          (*   return 0;    *)
 Define `w2_0 = (EL 0 g2.nodes)`; Define `w2_1 = (EL 1 g2.nodes)`; Define `r2_2 = (EL 2 g2.nodes)`;
 Define `r2_3 = (EL 3 g2.nodes)`; Define `w2_4 = (EL 4 g2.nodes)`;
 
 (* All the arrows defined in the example's diagram: *)
-val cg0_rel0 = prove( ``sequencedBefore g2 w2_0 cw0_1``,EVAL_TAC);
-val cg0_rel1 = prove( ``sequencedBefore g2 w2_1 cr0_2``,EVAL_TAC);
-val cg0_rel2 = prove( ``sequencedBefore g2 w2_1 cr0_3``,EVAL_TAC);
-val cg0_rel3 = prove( ``sequencedBefore g2 r2_2 cw0_4``,EVAL_TAC);
-val cg0_rel4 = prove( ``sequencedBefore g2 r2_3 cw0_4``,EVAL_TAC);
+val cg0_rel0 = prove( ``sequencedBefore g2 w2_0 w2_1``,EVAL_TAC);
+val cg0_rel1 = prove( ``sequencedBefore g2 w2_1 r2_2``,EVAL_TAC);
+val cg0_rel2 = prove( ``sequencedBefore g2 w2_1 r2_3``,EVAL_TAC);
+val cg0_rel3 = prove( ``sequencedBefore g2 r2_2 w2_4``,EVAL_TAC);
+val cg0_rel4 = prove( ``sequencedBefore g2 r2_3 w2_4``,EVAL_TAC);
 
 val sb_general_0 = prove(
   ``∀ nd g. ~(sequencedBefore g nd nd)``,
@@ -142,50 +151,60 @@ val sb_general_1 = prove(
   ``∀ g nd1 nd2. (sequencedBefore g nd1 nd2) ==> ~(sequencedBefore g nd2 nd1)``,
       RW_TAC arith_ss [sequencedBefore_def,sameThread_def,orderedBefore_def]);
 
+(* }}} *)
 
 (*        _                  ___                                 ___   __ 
   _ _ ___| |___ __ _ ___ ___/ __| ___ __ _ _  _ ___ _ _  __ ___ / _ \ / _|
  | '_/ -_) / -_) _` (_-</ -_)__ \/ -_) _` | || / -_) ' \/ _/ -_) (_) |  _|
  |_| \___|_\___\__,_/__/\___|___/\___\__, |\_,_\___|_||_\__\___|\___/|_|  
                                         |_|                                *)
+(* {{{ *)
 
 val rs_sanity_0 = prove(``∀ A B C g. ( (readsFrom g C B) ∧ (inReleaseSequenceOf g B A)) ==> (orderedBefore g A C)``,
                         METIS_TAC [sequencedBefore_def,
                                    inReleaseSequenceOf_def,
                                    readsFrom_def,AND_IMP_INTRO,
-                                   ob_sanity_5]);
+                                   ob_gen5]);
 
 val rs_sanity_1 = prove(``∀ A B g. ((inReleaseSequenceOf g A B) ∧ (A <> B)) ==> (orderedBefore g B A)``, RW_TAC(srw_ss()) [inReleaseSequenceOf_def,sequencedBefore_def]);
 
 val rs_sanity_2 = prove(``∀ A g. (inReleaseSequenceOf g A A)``, RW_TAC (srw_ss()) [inReleaseSequenceOf_def]);
+
+(* }}} *)
 
 (*                _        ___                        _                 _____    
   __ __ _ _ _ _ _(_)___ __|   \ ___ _ __  ___ _ _  __| |___ _ _  __ _  |_   _|__ 
  / _/ _` | '_| '_| / -_|_-< |) / -_) '_ \/ -_) ' \/ _` / -_) ' \/ _| || || |/ _ \
  \__\__,_|_| |_| |_\___/__/___/\___| .__/\___|_||_\__,_\___|_||_\__|\_, ||_|\___/
                                    |_|                              |__/         *)
+(* {{{ *)
 
-Define `g4'= FOLDL (receive') empty
+Define `g4= FOLDL (receive') empty
          [
-            ( Read  10 2   ACQUIRE    {} , 1) ;
-            ( Write 20 3   RELAXED   {2} , 1)
+            ( Read  10 0       ACQUIRE    {} , 1) ;
+            ( Write 20 1 (n 1) RELAXED   {0} , 1)
 ]`;
-Define `r4_0 = (EL 0 g4'.nodes)`; Define `w4_1 = (EL 1 g4'.nodes)`;
+Define `r4_0 = (EL 0 g4.nodes)`; Define `w4_1 = (EL 1 g4.nodes)`;
 
+val cd_rel0 = prove(``carriesDependencyTo g4 r4_0 w4_1``, EVAL_TAC);
 
+val cd_self = prove(``! g nd. ~carriesDependencyTo g nd nd``, RW_TAC (srw_ss()) [carriesDependencyTo_def,ob_gen3]);
+
+(* }}} *)
 
 (*                _                 _          __      ___ _   _    
   ____  _ _ _  __| |_  _ _ ___ _ _ (_)______ __\ \    / (_) |_| |_  
  (_-< || | ' \/ _| ' \| '_/ _ \ ' \| |_ / -_|_-<\ \/\/ /| |  _| ' \ 
  /__/\_, |_||_\__|_||_|_| \___/_||_|_/__\___/__/ \_/\_/ |_|\__|_||_|
      |__/                                                            *)
+(* {{{ *)
 
 Define `g5'= FOLDL (receive') empty
          [
-            ( Write 10 0 1 NOT_ATOMIC {} , 0) ;
-            ( Write 20 1 1 RELEASE    {} , 0) ;
-            ( Read  20 2   ACQUIRE    {} , 1) ;
-            ( Read  10 3   NOT_ATOMIC {} , 1)
+            ( Write 10 0 (n 1) NOT_ATOMIC {} , 0) ;
+            ( Write 20 1 (n 1) RELEASE    {} , 0) ;
+            ( Read  20 2       ACQUIRE    {} , 1) ;
+            ( Read  10 3       NOT_ATOMIC {} , 1)
 ]`;
 Define `w5_0 = (EL 0 g5'.nodes)`; Define `w5_1 = (EL 1 g5'.nodes)`;
 Define `r5_2 = (EL 2 g5'.nodes)`; Define `r5_3 = (EL 3 g5'.nodes)`;
@@ -206,9 +225,6 @@ val sw_rel4 = prove(``(happensBefore g5 w5_0 r5_3)``,
                     METIS_TAC [sw_rel1, ithb_rules] );
 
 val sw_sanity0 = prove( `` ~(synchronizesWith g5 w5_0 w5_1) ``, EVAL_TAC);
-
-
-val ad_sanity_0 = prove( ``∀nd. (sameAddress nd nd)``, EVAL_TAC THEN RW_TAC (srw_ss()) []);
 
 (* SynchronizesWith *)
 val sw_sanity1 = prove(
@@ -249,156 +265,192 @@ val sw_sanity1 = prove(
               Cases_on `Z = X` THEN  METIS_TAC [readsFrom_def, ob_gen3, ob_gen4, ob_gen5, rs_sanity_1]]
       ]);*)
 
+(* }}} *)
 
 (*   _           ___         _                _ ___       __             
   __| |___ _ __ / _ \ _ _ __| |___ _ _ ___ __| | _ ) ___ / _|___ _ _ ___ 
  / _` / -_) '_ \ (_) | '_/ _` / -_) '_/ -_) _` | _ \/ -_)  _/ _ \ '_/ -_)
  \__,_\___| .__/\___/|_| \__,_\___|_| \___\__,_|___/\___|_| \___/_| \___|
           |_|                                                             *)
+(* {{{ *)
 
-Define `g4'= FOLDL (receive') empty
+Define `g6'= FOLDL (receive') empty
          [
-            ( Write 10 0 1 RELEASE    {} , 0) ;
-            ( Write 10 1 2 RELAXED    {} , 0) ;
-            ( Read  10 2   ACQUIRE    {} , 1) ;
-            ( Write 20 3   RELAXED   {2} , 1)
+            ( Write 10 0 (n 1) RELEASE    {} , 0) ;
+            ( Write 10 1 (n 2) RELAXED    {} , 0) ;
+            ( Read  10 2       ACQUIRE    {} , 1) ;
+            ( Write 20 3 (n 3) RELAXED   {2} , 1)
 ]`;
-Define `w4_0 = (EL 0 g4'.nodes)`; Define `w4_1 = (EL 1 g4'.nodes)`;
-Define `r4_2 = (EL 2 g4'.nodes)`; Define `r4_3 = (EL 3 g4'.nodes)`;
-Define `g4 = resolve' g4' r4_2 w4_1`; 
+Define `w6_0 = (EL 0 g6'.nodes)`; Define `w6_1 = (EL 1 g6'.nodes)`;
+Define `r6_2 = (EL 2 g6'.nodes)`; Define `r6_3 = (EL 3 g6'.nodes)`;
+Define `g6 = resolve' g6' r6_2 w6_1`; 
+(*
+val do_rel0 = prove(``dependencyOrderedBefore g6 w6_1 r6_2``, 
+                   );
 
-
-val do_sanity0 = prove(
-    `` ∀ nd g. ~dependencyOrderedBefore g nd nd``,
-    
+val do_self = prove(`` ∀ nd g. ~dependencyOrderedBefore g nd nd``,
+                   );
+*)
+(* }}} *)
 
 (*_     _           _  _                             ___       __             
  (_)_ _| |_ ___ _ _| || |__ _ _ __ _ __  ___ _ _  __| _ ) ___ / _|___ _ _ ___ 
  | | ' \  _/ -_) '_| __ / _` | '_ \ '_ \/ -_) ' \(_-< _ \/ -_)  _/ _ \ '_/ -_)
  |_|_||_\__\___|_| |_||_\__,_| .__/ .__/\___|_||_/__/___/\___|_| \___/_| \___|
                              |_|  |_|                                          *)
+(* {{{ *)
 
-EVAL ``(sameThread
+Define `g7'= FOLDL (receive') empty
+         [
+            ( Write 10 0 (n 1) NOT_ATOMIC {} , 0) ;
+            ( Write 20 1 (n 1) RELEASE    {} , 0) ;
+            ( Read  20 2       ACQUIRE    {} , 1) ;
+            ( Read  10 3       NOT_ATOMIC {} , 1)
+]`;
+
+open lcsymtacs
+
+val ithb_obf = prove(
+`` ∀ g X Y. interthreadHappensBefore g X Y ==> orderedBefore g X Y``,
+cheat);
+  (*  Induct_on `interthreadHappensBefore` >>
+              metis_tac[orderedBefore_TRANS, sequencedBefore_obf,
+                        syncWith_obf])
+              MATCH_MP_TAC ithb_ind
+
+
 
 val it_sanity0 = prove(
-    `` ∀ nd g. ~ interthreadHappensBefore g nd nd ``,
+`` ∀ nd g. ~ interthreadHappensBefore g nd nd ``,
+metis_tac[ithb_obf, obf_IRREFL]
+
+         
     RW_TAC (srw_ss()) [ithb_rules] THEN
     `~synchronizesWith g nd nd` by METIS_TAC [sw_sanity1]
     `~dependencyOrderedBefore g nd nd` by METIS_TAC [dob_rules]
-    ...
+    ...);
 
+*)
+
+
+ 
+ (* }}} *)
+    
 (*_                                ___       __             
  | |_  __ _ _ __ _ __  ___ _ _  __| _ ) ___ / _|___ _ _ ___ 
  | ' \/ _` | '_ \ '_ \/ -_) ' \(_-< _ \/ -_)  _/ _ \ '_/ -_)
  |_||_\__,_| .__/ .__/\___|_||_/__/___/\___|_| \___/_| \___|
            |_|  |_|                                          *)
+(* {{{ *)
 
-(* Only sequencedBefore for now - too trivial. Should check other cases. *)
-Define `g6 = FOLDL (receive') empty
+Define `g8 = FOLDL (receive') empty
          [
-            ( Write 1024 0 112 SEQ_CST    {} , 1) ;
-            ( Read  1024 1     SEQ_CST    {} , 1) ;
-            ( Write 1024 2 10  SEQ_CST    {} , 1)
+            ( Write 1024 0 (n 11) SEQ_CST    {} , 1) ;
+            ( Read  1024 1        SEQ_CST    {} , 1) ;
+            ( Write 1024 2 (n 10) SEQ_CST    {} , 1)
          ]`;
-Define `w0_0 = (EL 0 g6.nodes)`; Define `r0_1 = (EL 1 g6.nodes)`; Define `w0_2 = (EL 2 g6.nodes)`;
+Define `w8_0 = (EL 0 g8.nodes)`; Define `r8_1 = (EL 1 g8.nodes)`; Define `w8_2 = (EL 2 g8.nodes)`;
 
 
 
 
 
-val hb_sanity_0 = prove(
-    `` happensBefore g0 w0_0 r0_1``,
-    EVAL_TAC);
+val hb_sanity_0 = prove( `` happensBefore g8 w8_0 r8_1``, EVAL_TAC);
 
 
 
 
 
 
-(* happensBefore *)
+(*
 g `∀ nd g. ~(happensBefore g nd nd)`;
 METIS_TAC [happensBefore_def, sequencedBefore_def, orderedBefore_def, sameThread_def
 
 RW_TAC arith_ss [happensBefore_def,sequencedBefore_def,orderedBefore_def, sameThread_def]
 RW_TAC arith_ss [ithb_rules]
+*)
 
-
+(* }}} *)
 
 (*    _    _ _    _    _____    
  __ _(_)__(_) |__| |__|_   _|__ 
  \ V / (_-< | '_ \ / -_)| |/ _ \
-  \_/|_/__/_|_.__/_\___||_|\___/
-                                 *)
+  \_/|_/__/_|_.__/_\___||_|\___/ *)
 
-Define `g7= FOLDL (receive') empty
+(* {{{ *)
+
+Define `g9= FOLDL (receive') empty
          [
-            ( Write 10 0 1 NOT_ATOMIC    {} , 0) ;
-            ( Write 10 1 2 NOT_ATOMIC    {} , 0) ;
-            ( Read  10 2   NOT_ATOMIC    {} , 1)
+            ( Write 10 0 (n 1) NOT_ATOMIC    {} , 0) ;
+            ( Write 10 1 (n 2) NOT_ATOMIC    {} , 0) ;
+            ( Read  10 2       NOT_ATOMIC    {} , 1)
 ]`;
-Define `w7_0 = (EL 0 g7.nodes)`; Define `w7_1 = (EL 1 g7.nodes)`;
-Define `r7_2 = (EL 2 g7.nodes)`;
+Define `w9_0 = (EL 0 g9.nodes)`; Define `w9_1 = (EL 1 g9.nodes)`;
+Define `r9_2 = (EL 2 g9.nodes)`;
+
+(* }}} *)
 
 (*    _    _ _    _     ___                                 ___   __ 
  __ _(_)__(_) |__| |___/ __| ___ __ _ _  _ ___ _ _  __ ___ / _ \ / _|
  \ V / (_-< | '_ \ / -_)__ \/ -_) _` | || / -_) ' \/ _/ -_) (_) |  _|
   \_/|_/__/_|_.__/_\___|___/\___\__, |\_,_\___|_||_\__\___|\___/|_|  
                                    |_|                                *)
+(* {{{ *)
 
-
-(* Incomplete: *)
+(* Incomplete:
 val in_own_release_seq = prove(
 ``∀ g nd. (MEM nd g.nodes) ==> (releaseSequenceOf g nd nd)``,
 RW_TAC arith_ss [releaseSequenceOf_def]
     RW_TAC arith_ss [releaseSequenceOf_def,modifiesBefore_def,isAtomic_def,isStore_def,sequencedBefore_def,orderedBefore_def,sameAddress_def,sameThread_def] THEN
 
+    
 e(DISCH_TAC ``orderedBefore g nd1 nd2``);
 
 e(`nd1.thread_id = nd2.thread_id` by METIS_TAC []);
 
 e(Cases_on `SOME x'`);
 e(RW_TAC arith_ss []  );
+ *)
 
-
-
+(* }}} *)
 
 (*             ___             _ ___              
   __ __ _ _ _ | _ \___ __ _ __| | __| _ ___ _ __  
  / _/ _` | ' \|   / -_) _` / _` | _| '_/ _ \ '  \ 
  \__\__,_|_||_|_|_\___\__,_\__,_|_||_| \___/_|_|_|
                                                    *)
+(* {{{ *)
 
-
-Define `g0= FOLDL (receive') <| nodes:=[]; rf:=FEMPTY |>
+Define `g11= FOLDL (receive') <| nodes:=[]; rf:=FEMPTY |>
          [
-            ( Write 1024 0 112 SEQ_CST    {} , 1) ;
-            ( Read  1024 1     SEQ_CST    {} , 1) ;
-            ( Write 1024 2 10  SEQ_CST    {} , 1)
+            ( Write 1024 0 (n 11) SEQ_CST    {} , 1) ;
+            ( Read  1024 1        SEQ_CST    {} , 1) ;
+            ( Write 1024 2 (n 10)  SEQ_CST    {} , 1)
          ]`;
-Define `w0_0 = (EL 0 g0.nodes)`; Define `r0_1 = (EL 1 g0.nodes)`; Define `w0_2 = (EL 2 g0.nodes)`;
-
-g `canReadFrom g0 r0_1 w0_0 = T`;
+Define `w11_0 = (EL 0 g11.nodes)`; Define `r11_1 = (EL 1 g11.nodes)`; Define `w11_2 = (EL 2 g11.nodes)`;
+(*
+g `canReadFrom g11 r11_1 w11_0 = T`;
 e (RW_TAC arith_ss [canReadFrom_def,isAtomic_def]);
-e (`r0_1.order <> NOT_ATOMIC` by EVAL_TAC );
-e (UNDISCH_TAC ``r0_1.order <> NOT_ATOMIC``);
+e (`r11_1.order <> NOT_ATOMIC` by EVAL_TAC );
+e (UNDISCH_TAC ``r11_1.order <> NOT_ATOMIC``);
 
 e (RW_TAC arith_ss [canReadFrom_def, isAtomic_def,visibleTo_def,happensBefore_def,sequencedBefore_def,orderedBefore_def]);
 
-e (`w0_1.order = SEQ_CST` by EVAL_TAC);
+e (`w11_1.order = SEQ_CST` by EVAL_TAC);
 e (EVAL_TAC);
 e (RW_TAC arith_ss []);
-e (`w1_2.order = SEQ_CST` by PROVE_TAC [] );
+e (`w11_2.order = SEQ_CST` by PROVE_TAC [] );
 
 
-e (Cases_on `w1_2.order` THEN Cases_on `r1_3.order`);
+e (Cases_on `w11_2.order` THEN Cases_on `r11_3.order`);
 (* HOW DO I SIMPLIFY w1_2.order to SEQ_CST? *)
 e (SIMP_TAC (srw_ss()) [node_accessors, memoryorder_distinct]);
 (*e (`w1_2.order <> NOT_ATOMIC` by DECIDE_TAC);*)
 
 
-g `inVisibleSequenceOf g0 r1_3 w1_2`;
+g `inVisibleSequenceOf g11 r11_3 w11_2`;
 e (RW_TAC (srw_ss()) [inVisibleSequenceOf_def]);
-
+*)
 
 (*
 Hand written:
@@ -421,16 +473,14 @@ Hand written:
 
 *)
 
-
-
-
+(* }}} *)
 
 (*___ ___ ___     ___ ___ _____ 
  / __| __/ _ \   / __/ __|_   _|
  \__ \ _| (_) | | (__\__ \ | |  
- |___/___\__\_\  \___|___/ |_|  
- 
- SEQ_CST                                *)
+ |___/___\__\_\  \___|___/ |_|   *)
+
+(* {{{ *)
 
 (*
 int main() {
@@ -446,11 +496,11 @@ int main() {
 
 Define `cg4= FOLDL (receive') empty
          [
-           ( Write 10 0 2 SEQ_CST       {} , 0 ) ;
-           ( Write 20 1 2 NOT_ATOMIC    {} , 0 ) ;
+           ( Write 10 0 (n 2) SEQ_CST       {} , 0 ) ;
+           ( Write 20 1 (n 2) NOT_ATOMIC    {} , 0 ) ;
            ( Read  10 2   SEQ_CST       {} , 2 ) ;
-           ( Write 10 3 3 SEQ_CST       {} , 1 ) ;
-           ( Write 20 4 0 NOT_ATOMIC   {3} , 2 )
+           ( Write 10 3 (n 3) SEQ_CST       {} , 1 ) ;
+           ( Write 20 4 (n 0) NOT_ATOMIC   {3} , 2 )
          ]`;
 
 Define `cw4_0 = (EL 0 cg4.nodes)`;
@@ -463,10 +513,13 @@ Define `cw4_4 = (EL 4 cg4.nodes)`;
 val cg4_rel0 = prove( ``sequencedBefore cg4 cw4_0 cw4_1``,EVAL_TAC );
 val cg4_rel2 = prove( ``sequencedBefore cg4 cr4_2 cw4_4``, EVAL_TAC );
 
-
+(*
 val cg4_rel1 = prove(
       ``sequentiallyConsistent cg4 cw4_0 cr4_2``,
       RW_TAC (srw_ss()) [sequentiallyConsistent_def]
       ...
+*)
 
-
+(* }}} *)
+      
+val _ = export_theory();
