uvmSystemScript.sml
@@ -1,0 +1,9 @@
+open HolKernel Parse boolLib bossLib;
+
+open uvmMemoryModelTheory;
+open uvmThreadSemanticsTheory;
+
+val _ = new_theory "uvmSystem";
+
+
+val _ = export_theory();
