uvmValuesScript.sml
@@ -1,0 +1,56 @@
+open HolKernel Parse boolLib bossLib;
+
+open uvmTypesTheory;
+
+val _ = new_theory "uvmValues";
+
+val _ = type_abbrev("addr", ``:num``)  (* non-local memory addresses *)
+
+(*tmp: ==========================================================*)
+val _ = type_abbrev("float32", ``:num``)
+val _ = type_abbrev("float64", ``:num``)
+val _ = type_abbrev("int",     ``:num``)
+(*===============================================================*)
+
+
+val _ = Datatype`
+   value =
+     Int num int
+   | IRef uvmType addr
+   | FloatV float32
+   | DoubleV float64
+   (* not sure if these are storable-in-register values
+   | StructV (value list)
+   | ArrayV (value list)
+   | Hybrid (value list) (value list) *)
+   | VectorV (value list)
+   | FuncRefV addr
+   | UFuncRefV addr
+`;
+
+val value_add_def = Define`
+value_add v1 v2 =
+     case (v1, v2) of
+         (Int n1 sz1, Int n2 sz2) => if sz1 = sz2 then SOME (Int (n1 + n2) sz1)
+                                     else NONE
+      |  (Int _ _, _) => NONE
+      | _ => NONE
+`;
+val _ = overload_on ("+", ``value_add``);
+
+val value_div_def = Define`
+    value_div v1 v2 =
+             case (v1,v2) of
+                 (Int n1 sz1, Int n2 sz2) => if (sz2=sz1 ∧ n2<>0) then SOME (Int (n1 DIV n2) sz1)
+                                             else NONE
+               | _ => NONE
+`;
+val _ = overload_on ("DIV", ``value_div``);
+
+val value_to_address = Define`
+    value_to_address (v:value) : (addr option) = case v of
+        Int n1 sz1 => SOME n1
+      | _ => NONE
+`;
+                    
+val _ = export_theory();
